–£—Å–ª–æ–≤–∏–µ:
–î–æ–∫–∞–∂–∏—Ç–µ, —á—Ç–æ –µ—Å–ª–∏ —Ñ—É–Ω–∫—Ü–∏—è $f(x)$ –Ω–µ–ø—Ä–µ—Ä—ã–≤–Ω–∞ –Ω–∞ $[-1, 1]$, –∏ –¥–ª—è –∫–∞–∂–¥–æ–π –Ω–µ–ø—Ä–µ—Ä—ã–≤–Ω–æ–π –Ω–∞ $[-1, 1]$ —á–µ—Ç–Ω–æ–π —Ñ—É–Ω–∫—Ü–∏–∏ $g(x)$:
$$\int_{-1}^{1} f(x)g(x) \, dx = 0$$
—Ç–æ —Ñ—É–Ω–∫—Ü–∏—è $f(x)$ –Ω–µ—á–µ—Ç–Ω–∞.

–î-–≤–æ:
–ó–∞–º–µ—Ç–∏–º, —á—Ç–æ ü§ì
$$f(x) = f_{e}(x) + f_{o}(x), ~~~ f_{e}(x) = \dfrac{f(x) + f(-x)}{2}, ~~~ f_{o}(x) = \dfrac{f(x) - f(-x)}{2}$$
–≥–¥–µ $f_{e}(x)$ - —á—ë—Ç–Ω–∞—è –∏ –Ω–µ–ø—Ä–µ—Ä—ã–≤–Ω–∞, $f_{o}(x)$ - –Ω–µ—á—ë—Ç–Ω–∞—è –∏ –Ω–µ–ø—Ä–µ—Ä—ã–≤–Ω–∞. –¢–æ–≥–¥–∞:
$$\int_{-1}^{1} f(x)g(x) \, dx = \int_{-1}^{1} (f_{e}(x) + f_{o}(x))g(x) \, dx = \int_{-1}^{1} f_{e}(x)g(x) \, dx + \int_{-1}^{1} f_{o}(x)g(x) \, dx $$
–°–¥–µ–ª–∞–µ–º –∑–∞–º–µ–Ω—É:
$$\int_{-1}^{1} f_{e}(x)g(x) \, dx + \int_{-1}^{1} f_{o}(x)g(x) \, dx = \begin{bmatrix}
t = -x & 1 \to -1 \\ 
dt = -dx & -1 \to 1
\end{bmatrix} = -\int_{1}^{-1} f_{e}(-t)g(-t) \, dt - \int_{1}^{-1} f_{o}(-t)g(-t) \, dt =$$
$$= \int_{-1}^{1} f_{e}(t)g(t) \, dt - \int_{-1}^{1} f_{o}(t)g(t) \, dt = 0$$
–ù–æ —Ç–∞–∫ –∫–∞–∫ $f_{o}(t)$ –Ω–µ—á—ë—Ç–Ω–∞ –∏ $g(t)$ —á—ë—Ç–Ω–∞:
$$\int_{-1}^{1} f_{o}(x)g(x) \, dx = 0$$
–ó–Ω–∞—á–∏—Ç:
$$\int_{-1}^{1} f_{e}(x)g(x) \, dx = 0$$
–í –∫–∞—á–µ—Å—Ç–≤–µ $g(x)$ –≤–æ–∑—å–º—ë–º $g(x) = f_{e}(x)$ –∏ —Ç–æ–≥–¥–∞:
$$\int_{-1}^{1} f_{e}^{2}(x) \, dx = 0$$
–ü–æ –Ω–µ–≤—ã—Ä–æ–∂–¥–µ–Ω–Ω–æ—Å—Ç–∏ –ø–æ–ª—É—á–∞–µ–º, —á—Ç–æ $f_{e}(x) = 0$, –∞ –∑–Ω–∞—á–∏—Ç $f(x) = f_{o}(x)$ –∏ $f(x)$ –Ω–µ—á—ë—Ç–Ω–∞.