## Алгебраическая теорема Вейерштрасса
Формулировка:
$\forall{f(x)}~-$ непрерывна на $[a,b]$
$\exists{\{P_{n}(x)\}}_{n=1}^{\infty}~~P_{m}(x) = \sum_{k=1}^{n} a_{k}x^{k}~~~~~P_{n}(x) \rightrightarrows_{n \to \infty}^{[a,b]} f(x)$
$\forall{\varepsilon>0}~~\exists{N}~~\forall{n>N}~~\forall{x \in [a,b]}\mathpunct{:}$
$$|P_{n}(x)-f(x)|<\varepsilon$$
Д-во (Бернштейна):
$b_{n,k} = x^{k}(1-x)^{n-k},~~~~n \in N, k = 0,1,2,3\dots n$
$b^{'}_{n,k} = x^{k-1}(1-x)^{n-k-1}$
$(k(1-x) - (1-x))^{n-k-1}$
$x = 0,~x=1~-min$
$k-kx-xn-kx=k-xn=0,~~~x=\dfrac{k}{n}~- \max$
$1.$ Пусть $[a,b] = [0,1]$
$B_{n}(x) = \sum_{k=0}^{n} C_{n}^{k} x^{k}(1-x)^{n-k}$
$P_{n}(x) = \sum_{k=0}^{n} f\left( \dfrac{k}{n} \right) * b_{n,k} (x)$

## Лемма
Формулировка:
1) $\sum_{k=1}^{n} b_{n,k}(x)=1$
2) $\sum_{k=1}^{n} \dfrac{k}{n} b_{n,k} (x) = x$
3) $\sum_{k=1}^{n} \left( \dfrac{k}{n}  - x \right)^{2} - b_{n,k}(x) = \dfrac{x(1-x)}{n}$

Д-во:
${} 1.~ {}$$\sum_{k=-0}^{n} C_{n}^{k} x^{k} (1-x)^{n-k} = (x+(1-x))^{n} = 1^{n} = 1$
$2.~$$\sum_{k=-0}^{n} \dfrac{k}{n} C_{n}^{k} x^{k} (1-x)^{n-k}=$
$=\sum_{k=0}^{n} \dfrac{k}{n} * \dfrac{n!}{k!(n-k)!} x^{k}(1-x)^{n-k}$
$= x \sum_{k=0}^{n} \dfrac{(n-1)!}{(k-1)!(n-k)!} x^{k-1}(1-x)^{n-k}=$
$= x \sum_{k=0}^{n} \dfrac{(n-1)!}{k!(n-1-k)!} x^{k}(1-x)^{n-1-k} =$
$= x \sum_{k=0}^{n} C^{k}_{n} x^{k} (1-x)^{n-1-k}$
$3.~$$\left( \sum_{k=0}^{n} \left( \dfrac{k}{n} -x \right) b_{n,k}(x) \right) = 0$
$-\sum_{k=0}^{n} b_{n,k}(x) + \sum_{k=0}^{n} \left( \dfrac{k}{n} - x \right)^{2} b_{n,k}(x) \dfrac{n}{x(1-x)} = 0$
Что такое $b_{n,k}\mathpunct{:}~~$
$$b_{n,k} = C_{n}^{k} (k-nx)x^{k-1}(1-x)^{n-k-1} = C_{n}^{k} x^{k}(1-x)^{n-k} \left( \dfrac{k}{n} -x \right) \dfrac{n}{x(1-x)}$$
