Формулировка: 
${} \{X_{n} \notin 0\},~x_{n} \to 0 \mathpunct{:}~~ A(x) = \sum_{k=0}^{\infty} a_{k}x^{k}\mathpunct{;}~~B(x) = \sum_{k=0}^{\infty} b_{k}x^{k} {}$
Пусть $A(x_{n}) = B(x_{n})\mathpunct{:}~~\forall{n \in \mathbb{N}}~~$тогда $a_{k} = b_{k}~~\forall{k \in \mathbb{N}}~~$

Д-во:
$$\lim_{n \to \infty} \sum_{k=0}^{\infty} a_{k} x_{n}^{k} = \lim_{n \to \infty} \sum_{k=0}^{\infty} b_{k} x_{n}^{k} \Rightarrow a_{0} = b_{0}$$
Если $x_{1} \neq 0$ и $A(x_{1})$ и $B(x_{1})$ сходится, то $R \geq |x_{1}|,$ тогда $\forall{|x_{n}| < R}~~$сходится равномерно оба ряда
$$a_{0} + \sum_{k=1}^{\infty} a_{k} x_{n}^{k} = b_{0} + \sum_{k=1}^{\infty} b_{k} x_{n}^{k}~| \mathpunct{:}x_{n} \neq 0$$
$$\lim_{n \to \infty} \sum_{k=1}^{\infty} a_{k}x^{k-1}_{n} = \lim_{n \to \infty} \sum_{k=1}^{\infty} b_{k}x^{k-1}_{n} \Rightarrow a_{1} = b_{1}~~~~\square$$



