## Признак Лейбница 
Формулировка:
```spoiler-markdown
Если $a_{n} > 0,~$ $a_{n} \to 0$ монотонно, тогда $\sum_{n=1}^{\infty} (-1)^{n} a_{n}$ причем $|R_{n}| = |S - S_{n}| \leq a_{n+1}$
```

Д-во:
```spoiler-markdown
$S_{2n-1} = a_{1} - a_{2} + a_{3} - a_{4} +a_{5} -\dots+ a_{2n-1}$
$S_{2n+1} - S_{2n-1} = a_{2n+1} - a_{2n} < 0,~~~~\{S_{2n-1}\}~-$ убывает
$\Rightarrow \{S_{2n-1}\}^{\infty}_{n = 1}~-$ сходиться $\Rightarrow$ $S_{2n-1} \rightarrow_{n \to \infty} S$
$S_{2n} = S_{2n-1} - a_{2n} \to_{n \to \infty} S\mathpunct{:}~~S_{n} \to_{n \to \infty} S$ т.е ряд сходиться 
$\square$
```
## Признак Абеля 
Формулировка:
```spoiler-markdown
Если $\sum_{n=1}^{\infty} a_{n}~-$ сходится, $b_{n} \to_{n \to \infty} b$ монотонно, тогда $\sum_{n=1}^{\infty} a_{n} b_{n}~-$ сходиться
```

Д-во:
```spoiler-markdown
$c_{n} = b_{n} - b \to 0$ монотонно 
$\sum_{n=1}^{\infty} a_{n} \Rightarrow A_{n} = \sum_{k=1}^{n} a_{k}~-$ ограниченна
$\Rightarrow \sum_{n=1}^{\infty} a_{n}b_{n} = \sum_{n=1}^{\infty} a_{n}(b_{n} - b) + \sum_{n=1}^{\infty} a_{n}b$
$\sum_{n=1}^{\infty} a_{n}(b_{n} - b)~-$ сходится по признаку Дирихле
$\sum_{n=1}^{\infty} a_{n}b~-$ сходится по монотонности
$\square$
```
## Признак Дирихле
Формулировка:
```spoiler-markdown
Если $A_{k} = \sum_{k=0}^{n} a_{k}$ ограничен $(|A_{k}| \leq A)$
$b_{n} \to_{n \to \infty} 0$ монотонно, то $\sum_{n=1}^{\infty} a_{n}b_{n}~-$ сходится 
```

Д-во:
```spoiler-markdown
$\tilde{A}_{n} = \sum_{k=m+1}^{n} a_{k},~~n>m,~~m = 0~\tilde{A}_{m} = 0$
$a_{n} = \tilde{A}_{n} - \tilde{A}_{n-1}$
$$\sum_{k = m+1}^{n} a_{k}b_{k} = \sum_{k = m+1}^{n} (\tilde{A}_{k} - \tilde{A}_{k+1})b_{k} = \sum_{k = m+1}^{n} \tilde{A}_{k} b_{k} - \sum_{k = m+1}^{n} \tilde{A}_{k+1}b_{k}=$$
$$\sum_{k = m+1}^{n} \tilde{A}_{k}b_{k} - \sum_{k = m+1}^{n} \tilde{A}_{k}b_{k+1} + \tilde{A}_{n}b_{n} =$$
$$= \sum_{k = m+1}^{n} \tilde{A}_{k}(b_{k} - b_{k-1}) + \tilde{A}_{n}b_{n} - \tilde{A}_{m}b_{m+1}$$
- $b_{n} \to 0,~~\forall{\varepsilon>0}~~\exists{N}~~\forall{n > N}~~|b_{n}| < \dfrac{\varepsilon}{6A}$
 $$|\sum_{k = m+1}^{n}| \leq 2A(\sum_{k = m+1}^{n-1} |b_{k} - b_{k+1}| + |b_{n}|) \leq$$
 $$ \leq 2A(|b_{m+1}| + |b_{n}| + |b_{n}|) <$$
$$< 2A\left( \dfrac{\varepsilon}{6A} + \dfrac{\varepsilon}{6A} +\dfrac{\varepsilon}{6A} \right) = \varepsilon~~\square(кр.Коши)$$
```
